.

projects/SmullyanGIT/PA.v
@@ -8,7 +8,205 @@ Require Import DschingisKhan.pure.MyStructures.
 Require Import DschingisKhan.pure.MyUtilities.
 
 Module Tarski's_Theorem_for_Arithmetic.
-  
+
+  Import ListNotations MyUtilities MyUniverses.
+
+  Section BasicSyntaxDefn.
+
+  Definition Vr : Set :=
+    nat
+  .
+
+  Definition Vr_eq_dec : forall x : Vr, forall y : Vr, {x = y} + {x <> y} :=
+    Nat.eq_dec
+  .
+
+  Inductive Tm : Set :=
+  | ivarTm : forall x : Vr, Tm
+  | zeroTm : Tm
+  | succTm : forall t1 : Tm, Tm
+  | plusTm : forall t1 : Tm, forall tm2 : Tm, Tm
+  | multTm : forall t1 : Tm, forall tm2 : Tm, Tm
+  | expoTm : forall t1 : Tm, forall tm2 : Tm, Tm
+  .
+
+  Lemma Tm_eq_dec :
+    forall t1 : Tm,
+    forall t2 : Tm,
+    {t1 = t2} + {t1 <> t2}.
+  Proof with try ((right; congruence) || (left; congruence)).
+    induction t1; destruct t2...
+    - destruct (Vr_eq_dec x x0)...
+    - destruct (IHt1 t2)...
+    - destruct (IHt1_1 t2_1); destruct (IHt1_2 t2_2)...
+    - destruct (IHt1_1 t2_1); destruct (IHt1_2 t2_2)...
+    - destruct (IHt1_1 t2_1); destruct (IHt1_2 t2_2)...
+  Qed.
+
+  Inductive Form : Set :=
+  | eqnF : forall t1 : Tm, forall t2 : Tm, Form
+  | leqF : forall t1 : Tm, forall t2 : Tm, Form
+  | negF : forall f1 : Form, Form
+  | impF : forall f1 : Form, forall f2 : Form, Form
+  | allF : forall y : Vr, forall f1 : Form, Form
+  .
+
+  Lemma Form_eq_dec :
+    forall f1 : Form,
+    forall f2 : Form,
+    {f1 = f2} + {f1 <> f2}.
+  Proof with try ((right; congruence) || (left; congruence)).
+    induction f1; destruct f2...
+    - destruct (Tm_eq_dec t1 t0); destruct (Tm_eq_dec t2 t3)...
+    - destruct (Tm_eq_dec t1 t0); destruct (Tm_eq_dec t2 t3)...
+    - destruct (IHf1 f2)...
+    - destruct (IHf1_1 f2_1); destruct (IHf1_2 f2_2)...
+    - destruct (Vr_eq_dec y y0); destruct (IHf1 f2)...
+  Qed.
+
+  End BasicSyntaxDefn.
+
+  Section BasicSemanticsDefn.
+
+  Let VrValue : InferiorUniverse :=
+    nat
+  .
+
+  Definition Env : InferiorUniverse :=
+    Vr -> VrValue
+  .
+
+  Definition TmValue : InferiorUniverse :=
+    VrValue
+  .
+
+  Fixpoint evalTm (mathbfE : Env) (t : Tm) {struct t} : TmValue :=
+    match t with
+    | ivarTm x => mathbfE x
+    | zeroTm => O
+    | succTm t1 => S (evalTm mathbfE t1)
+    | plusTm t1 t2 => plus (evalTm mathbfE t1) (evalTm mathbfE t2)
+    | multTm t1 t2 => mult (evalTm mathbfE t1) (evalTm mathbfE t2)
+    | expoTm t1 t2 => Nat.pow (evalTm mathbfE t1) (evalTm mathbfE t2)
+    end
+  .
+
+  Definition FormValue : InferiorUniverse :=
+    Prop
+  .
+
+  Fixpoint evalForm (mathbfE : Env) (f : Form) {struct f} : FormValue :=
+    match f with
+    | eqnF t1 t2 => eq (evalTm mathbfE t1) (evalTm mathbfE t2)
+    | leqF t1 t2 => le (evalTm mathbfE t1) (evalTm mathbfE t2)
+    | negF f1 => ~ evalForm mathbfE f1
+    | impF f1 f2 => evalForm mathbfE f1 -> evalForm mathbfE f2
+    | allF y f1 => forall v : VrValue, evalForm (fun z : Vr => if Vr_eq_dec y z then v else mathbfE z) f1
+    end
+  .
+
+  End BasicSemanticsDefn.
+
+  Section OccurencesDefn.
+
+  Fixpoint occursFreeInTm (z : Vr) (t : Tm) {struct t} : bool :=
+    match t with
+    | ivarTm x => if Vr_eq_dec x z then true else false
+    | zeroTm => false
+    | succTm t1 => occursFreeInTm z t1
+    | plusTm t1 t2 => occursFreeInTm z t1 || occursFreeInTm z t2
+    | multTm t1 t2 => occursFreeInTm z t1 || occursFreeInTm z t2
+    | expoTm t1 t2 => occursFreeInTm z t1 || occursFreeInTm z t2
+    end
+  .
+
+  Fixpoint occursFreeInForm (z : Vr) (f : Form) {struct f} : bool :=
+    match f with
+    | eqnF t1 t2 => occursFreeInTm z t1 || occursFreeInTm z t2
+    | leqF t1 t2 => occursFreeInTm z t1 || occursFreeInTm z t2
+    | negF f1 => occursFreeInForm z f1
+    | impF f1 f2 => occursFreeInForm z f1 || occursFreeInForm z f2
+    | allF y f1 => if Vr_eq_dec y z then false else occursFreeInForm z f1
+    end
+  .
+
+  Fixpoint getFreeVarsTm (t : Tm) {struct t} : list Vr :=
+    match t with
+    | ivarTm x => [x]
+    | zeroTm => []
+    | succTm t1 => getFreeVarsTm t1
+    | plusTm t1 t2 => getFreeVarsTm t1 ++ getFreeVarsTm t2
+    | multTm t1 t2 => getFreeVarsTm t1 ++ getFreeVarsTm t2
+    | expoTm t1 t2 => getFreeVarsTm t1 ++ getFreeVarsTm t2
+    end
+  .
+
+  Fixpoint getFreeVarsForm (f : Form) {struct f} : list Vr :=
+    match f with
+    | eqnF t1 t2 => getFreeVarsTm t1 ++ getFreeVarsTm t2
+    | leqF t1 t2 => getFreeVarsTm t1 ++ getFreeVarsTm t2
+    | negF f1 => getFreeVarsForm f1
+    | impF f1 f2 => getFreeVarsForm f1 ++ getFreeVarsForm f2
+    | allF y f1 => remove Vr_eq_dec y (getFreeVarsForm f1)
+    end
+  .
+
+  End OccurencesDefn.
+
+  Section SubstitutionDefn.
+
+  Definition substitution: Set :=
+    Vr -> Tm
+  .
+
+  Definition nilSubst : substitution :=
+    ivarTm
+  .
+
+  Definition consSubst (x : Vr) (t : Tm) (sigma : substitution) : substitution :=
+    fun z : Vr =>
+    if Vr_eq_dec x z
+    then t
+    else sigma z
+  .
+
+  Definition applySubst_Vr (sigma : substitution) (x : Vr) : Tm :=
+    sigma x
+  .
+
+  Definition getMaxNumOfFreeVarsInTm (t : Tm) : Vr :=
+    fold_right_max_0 (getFreeVarsTm t)
+  .
+
+  Definition chi (sigma : substitution) (f : Form) : Vr :=
+    S (fold_right_max_0 (map (fun x : Vr => getMaxNumOfFreeVarsInTm (applySubst_Vr sigma x)) (getFreeVarsForm f)))
+  .
+
+  Fixpoint applySubst_Tm (sigma : substitution) (t : Tm) {struct t} : Tm :=
+    match t with
+    | ivarTm x => applySubst_Vr sigma x
+    | zeroTm => zeroTm
+    | succTm t1 => succTm (applySubst_Tm sigma t1)
+    | plusTm t1 t2 => plusTm (applySubst_Tm sigma t1) (applySubst_Tm sigma t2)
+    | multTm t1 t2 => multTm (applySubst_Tm sigma t1) (applySubst_Tm sigma t2)
+    | expoTm t1 t2 => expoTm (applySubst_Tm sigma t1) (applySubst_Tm sigma t2)
+    end
+  .
+
+  Fixpoint applySubst_Form (sigma : substitution) (f : Form) {struct f} : Form :=
+    match f with
+    | eqnF t1 t2 => eqnF (applySubst_Tm sigma t1) (applySubst_Tm sigma t2)
+    | leqF t1 t2 => leqF (applySubst_Tm sigma t1) (applySubst_Tm sigma t2)
+    | negF f1 => negF (applySubst_Form sigma f1)
+    | impF f1 f2 => impF (applySubst_Form sigma f1) (applySubst_Form sigma f2)
+    | allF x f1 =>
+      let z : Vr := chi sigma f in
+      allF z (applySubst_Form (consSubst x (ivarTm z) sigma) f1)
+    end
+  .
+
+  End SubstitutionDefn.
+
 End Tarski's_Theorem_for_Arithmetic.
 
 Module The_Incompleteness_of_Peano_Arithmetic_With_Exponentation.
